module P2 where

open import lists
open import F2

-- Round III

PredCtx : (γ : TyCtx) → Type₀
PredCtx = Ctx

PredPos : {γ : TyCtx} → PredCtx γ → Type₀
PredPos = CtxPos

PredVar : {γ : TyCtx} → PredCtx γ → Ty γ → Type₀
PredVar = Var

data Proposition : {γ : TyCtx} (Γ̂ : PredCtx γ) (Γ : Ctx γ) → Type₀

data Predicate : {γ : TyCtx} (Γ̂ : PredCtx γ) (Γ : Ctx γ) (A : Ty γ) → Type₀ where
  𝑃𝑉 : {γ : TyCtx} {Γ̂ : PredCtx γ} {Γ : Ctx γ} {A : Ty γ} →
    PredVar Γ̂ A → Predicate Γ̂ Γ A
  𝑃𝐿 : {γ : TyCtx} {Γ̂ : PredCtx γ} {Γ : Ctx γ} {Â : Ty γ} →
    Proposition Γ̂ (Γ ⊹ Â) → Predicate Γ̂ Γ Â

data Proposition where
  _∈_ : {γ : TyCtx} {Γ̂ : PredCtx γ} {Γ : Ctx γ} {A : Ty γ} →
    Tm Γ A → Predicate Γ̂ Γ A → Proposition Γ̂ Γ
  _⇛_ : {γ : TyCtx} {Γ̂ : PredCtx γ} {Γ : Ctx γ} →
    Proposition Γ̂ Γ → Proposition Γ̂ Γ → Proposition Γ̂ Γ
  ∀𝒳 : {γ : TyCtx} {Γ̂ : PredCtx γ} {Γ : Ctx γ} {Â : Ty γ} →
    Proposition (Γ̂ ⊹ Â) Γ → Proposition Γ̂ Γ
  ∀x : {γ : TyCtx} {Γ̂ : PredCtx γ} {Γ : Ctx γ} {A : Ty γ} →
    Proposition Γ̂ (Γ ⊹ A) → Proposition Γ̂ Γ
  ∀X : {γ : TyCtx} {Γ̂ : PredCtx γ} {Γ : Ctx γ} {⋆ : ⊤} →
    Proposition (shiftCtx {⋆ = ⋆} 𝑧𝑝 Γ̂) (shiftCtx 𝑧𝑝 Γ) → Proposition Γ̂ Γ

shiftProp-n : {γ : TyCtx} {Γ̂ : PredCtx γ} {Γ : Ctx γ}  {⋆ : ⊤}
  (𝑖 : TyPos γ) → Proposition Γ̂ Γ → Proposition (shiftCtx {⋆ = ⋆} 𝑖 Γ̂) (shiftCtx 𝑖 Γ)

shiftPred-n : {γ : TyCtx} {Γ̂ : PredCtx γ} {Γ : Ctx γ} {A : Ty γ}  {⋆ : ⊤}
  (𝑖 : TyPos γ) → Predicate Γ̂ Γ A → Predicate (shiftCtx {⋆ = ⋆} 𝑖 Γ̂) (shiftCtx 𝑖 Γ) (shiftTy 𝑖 A)
shiftPred-n 𝑖 (𝑃𝑉 v) = 𝑃𝑉 (shiftVar-γ 𝑖 v)
shiftPred-n 𝑖 (𝑃𝐿 𝐴) = 𝑃𝐿 (shiftProp-n 𝑖 𝐴)

shiftProp-n 𝑖 (t ∈ 𝒜) = shiftTm-γ 𝑖 t ∈ shiftPred-n 𝑖 𝒜
shiftProp-n 𝑖 (𝐴 ⇛ 𝐵) = shiftProp-n 𝑖 𝐴 ⇛ shiftProp-n 𝑖 𝐵
shiftProp-n 𝑖 (∀𝒳 𝐴) = ∀𝒳 (shiftProp-n 𝑖 𝐴)
shiftProp-n 𝑖 (∀x 𝐴) = ∀x (shiftProp-n 𝑖 𝐴)
shiftProp-n {Γ̂ = Γ̂} {Γ} 𝑖 (∀X 𝐴) = ∀X
  (tr (λ Γ → Proposition  (shiftCtx 𝑧𝑝 (shiftCtx 𝑖 Γ̂)) Γ) (shiftCtx² 𝑧𝑝 𝑖 Γ)
    (tr (λ Γ̂ → Proposition Γ̂ (shiftCtx (𝑠𝑝 𝑖) (shiftCtx 𝑧𝑝 Γ))) (shiftCtx² 𝑧𝑝 𝑖 Γ̂)
      (shiftProp-n (𝑠𝑝 𝑖) 𝐴)))

shiftProp-Γ̂ : {γ : TyCtx} {Γ̂ : PredCtx γ} {Γ : Ctx γ} {Â : Ty γ}
  (𝑖 : PredPos Γ̂) → Proposition Γ̂ Γ → Proposition (insert𝐶𝑡𝑥 𝑖 Â) Γ

shiftPred-Γ̂ : {γ : TyCtx} {Γ̂ : PredCtx γ} {Γ : Ctx γ} {Â A : Ty γ}
  (𝑖 : PredPos Γ̂) → Predicate Γ̂ Γ A → Predicate (insert𝐶𝑡𝑥 𝑖 Â) Γ A
shiftPred-Γ̂ 𝑖 (𝑃𝑉 v) = 𝑃𝑉 (shift𝑉𝑎𝑟 𝑖 v)
shiftPred-Γ̂ 𝑖 (𝑃𝐿 𝐴) = 𝑃𝐿 (shiftProp-Γ̂ 𝑖 𝐴)

shiftProp-Γ̂ 𝑖 (t ∈ 𝒜) = t ∈ shiftPred-Γ̂ 𝑖 𝒜
shiftProp-Γ̂ 𝑖 (𝐴 ⇛ 𝐵) = shiftProp-Γ̂ 𝑖 𝐴 ⇛ shiftProp-Γ̂ 𝑖 𝐵
shiftProp-Γ̂ 𝑖 (∀𝒳 𝐴) = ∀𝒳 (shiftProp-Γ̂ (𝑠𝑝 𝑖) 𝐴)
shiftProp-Γ̂ 𝑖 (∀x 𝐴) = ∀x (shiftProp-Γ̂ 𝑖 𝐴)
shiftProp-Γ̂ {Γ = Γ} 𝑖 (∀X 𝐴) =
  ∀X (tr (λ Δ → Proposition Δ (shiftCtx 𝑧𝑝 Γ)) (shiftInsert 𝑧𝑝 𝑖)
    (shiftProp-Γ̂ (shiftCtxPos-γ 𝑧𝑝 𝑖) 𝐴))

shiftProp-Γ : {γ : TyCtx} {Γ̂ : PredCtx γ} {Γ : Ctx γ} {A : Ty γ}
  (𝑖 : CtxPos Γ) → Proposition Γ̂ Γ → Proposition Γ̂ (insert𝐶𝑡𝑥 𝑖 A)

shiftPred-Γ : {γ : TyCtx} {Γ̂ : PredCtx γ} {Γ : Ctx γ} {A B : Ty γ}
  (𝑖 : CtxPos Γ) → Predicate Γ̂ Γ B → Predicate Γ̂ (insert𝐶𝑡𝑥 𝑖 A) B
shiftPred-Γ 𝑖 (𝑃𝑉 v) = 𝑃𝑉 v
shiftPred-Γ 𝑖 (𝑃𝐿 𝐴) = 𝑃𝐿 (shiftProp-Γ (𝑠𝑝 𝑖) 𝐴 )

shiftProp-Γ 𝑖 (t ∈ 𝒜) = shiftTm 𝑖 t ∈ shiftPred-Γ 𝑖 𝒜
shiftProp-Γ 𝑖 (𝐴 ⇛ 𝐵) = shiftProp-Γ 𝑖 𝐴 ⇛ shiftProp-Γ 𝑖 𝐵
shiftProp-Γ 𝑖 (∀𝒳 𝐴) = ∀𝒳 (shiftProp-Γ 𝑖 𝐴)
shiftProp-Γ 𝑖 (∀x 𝐴) = ∀x (shiftProp-Γ (𝑠𝑝 𝑖) 𝐴)
shiftProp-Γ {Γ̂ = Γ̂} 𝑖 (∀X 𝐴) =
  ∀X (tr (λ Δ → Proposition (shiftCtx 𝑧𝑝 Γ̂) Δ) (shiftInsert 𝑧𝑝 𝑖)
    (shiftProp-Γ (shiftCtxPos-γ 𝑧𝑝 𝑖) 𝐴))

subsPredInProp : {γ : TyCtx} {Γ̂ : PredCtx γ} {Γ : Ctx γ} {Â : Ty γ} →
  Proposition Γ̂ Γ → (v : PredVar Γ̂ Â) → Predicate (prefix𝑉𝑎𝑟 v) Γ Â → Proposition (remove𝑉𝑎𝑟 v) Γ

subsPredVar : {γ : TyCtx} {Γ̂ : PredCtx γ} {Γ : Ctx γ} {Â A : Ty γ} →
  PredVar Γ̂ A → (v : PredVar Γ̂ Â) → Predicate (prefix𝑉𝑎𝑟 v) Γ Â → Predicate (remove𝑉𝑎𝑟 v) Γ A
subsPredVar 𝑧𝑣 𝑧𝑣 𝒜 = 𝒜
subsPredVar 𝑧𝑣 (𝑠𝑣 v) 𝒜 = 𝑃𝑉 𝑧𝑣
subsPredVar (𝑠𝑣 w) 𝑧𝑣 𝒜 = 𝑃𝑉 w
subsPredVar (𝑠𝑣 w) (𝑠𝑣 v) 𝒜 = shiftPred-Γ̂ 𝑧𝑝 (subsPredVar w v 𝒜)

subsPredInPred : {γ : TyCtx} {Γ̂ : PredCtx γ} {Γ : Ctx γ} {Â A : Ty γ} →
  Predicate Γ̂ Γ A → (v : PredVar Γ̂ Â) → Predicate (prefix𝑉𝑎𝑟 v) Γ Â → Predicate (remove𝑉𝑎𝑟 v) Γ A
subsPredInPred (𝑃𝑉 w) v 𝒜 = subsPredVar w v 𝒜
subsPredInPred (𝑃𝐿 𝐴) v 𝒜 = 𝑃𝐿 (subsPredInProp 𝐴 v (shiftPred-Γ 𝑧𝑝 𝒜))

subsPredInProp (t ∈ ℬ) v 𝒜 = t ∈ (subsPredInPred ℬ v 𝒜)
subsPredInProp (𝐴 ⇛ 𝐵) v 𝒜 = subsPredInProp 𝐴 v 𝒜 ⇛ subsPredInProp 𝐵 v 𝒜
subsPredInProp (∀𝒳 𝐴) v 𝒜 = ∀𝒳 (subsPredInProp 𝐴 (𝑠𝑣 v) 𝒜)
subsPredInProp (∀x 𝐴) v 𝒜 = ∀x (subsPredInProp 𝐴 v (shiftPred-Γ 𝑧𝑝 𝒜))
subsPredInProp {Γ = Γ} {Â} (∀X 𝐴) v 𝒜 =
  ∀X (tr (λ Γ̂ → Proposition Γ̂ (shiftCtx 𝑧𝑝 Γ)) (shiftRemove 𝑧𝑝 v ⁻¹)
    (subsPredInProp 𝐴 (shiftVar-γ 𝑧𝑝 v)
      (tr (λ Γ̂ → Predicate Γ̂ (shiftCtx 𝑧𝑝 Γ) (shiftTy 𝑧𝑝 Â)) (shiftPrefix 𝑧𝑝 v)
        (shiftPred-n 𝑧𝑝 𝒜))))

subsTmInProp : {γ : TyCtx} {Γ̂ : PredCtx γ} {Γ : Ctx γ} {A : Ty γ} →
  Proposition Γ̂ Γ → (v : Var Γ A) → Tm (prefix𝑉𝑎𝑟 v) A  → Proposition Γ̂ (remove𝑉𝑎𝑟 v)

subsTmInPred : {γ : TyCtx} {Γ̂ : PredCtx γ} {Γ : Ctx γ} {A B : Ty γ} →
  Predicate Γ̂ Γ B → (v : Var Γ A) → Tm (prefix𝑉𝑎𝑟 v) A → Predicate Γ̂ (remove𝑉𝑎𝑟 v) B
subsTmInPred (𝑃𝑉 w) v t = 𝑃𝑉 w
subsTmInPred (𝑃𝐿 𝐴) v t = 𝑃𝐿 (subsTmInProp 𝐴 (𝑠𝑣 v) t)

subsTmInProp (s ∈ 𝒜) v t = subsTm s v t ∈ subsTmInPred 𝒜 v t
subsTmInProp (𝐴 ⇛ 𝐵) v t = subsTmInProp 𝐴 v t ⇛ subsTmInProp 𝐵 v t
subsTmInProp (∀𝒳 𝐴) v t = ∀𝒳 (subsTmInProp 𝐴 v t)
subsTmInProp (∀x 𝐴) v t = ∀x (subsTmInProp 𝐴 (𝑠𝑣 v) t)
subsTmInProp {Γ̂ = Γ̂} {Γ} {A} (∀X 𝐴) v t =
  ∀X (tr (λ Γ → Proposition (shiftCtx 𝑧𝑝 Γ̂) Γ) (shiftRemove 𝑧𝑝 v ⁻¹)
    (subsTmInProp 𝐴 (shiftVar-γ 𝑧𝑝 v)
      (tr (λ Γ → Tm Γ (shiftTy 𝑧𝑝 A)) (shiftPrefix 𝑧𝑝 v) (shiftTm-γ 𝑧𝑝 t))))

subsTyInProp : {γ : TyCtx} {⋆ : ⊤} {Γ̂ : PredCtx γ} {Γ : Ctx γ} →
  Proposition Γ̂ Γ → (v : TyVar γ ⋆) → (A : Ty (prefix𝑉𝑎𝑟 v)) →
  Proposition (subsCtx Γ̂ v A) (subsCtx Γ v A)

subsTyInPred : {γ : TyCtx} {⋆ : ⊤} {Γ̂ : PredCtx γ} {Γ : Ctx γ} {B : Ty γ} →
  Predicate Γ̂ Γ B → (v : TyVar γ ⋆) → (A : Ty (prefix𝑉𝑎𝑟 v)) →
  Predicate (subsCtx Γ̂ v A) (subsCtx Γ v A) (subsTy B v A)
subsTyInPred (𝑃𝑉 w) v A = 𝑃𝑉 (subsVar-γ w v A)
subsTyInPred (𝑃𝐿 𝐴) v A = 𝑃𝐿 (subsTyInProp 𝐴 v A )

subsTyInProp (t ∈ 𝒜) v A = subsTm-γ t v A ∈ subsTyInPred 𝒜 v A
subsTyInProp (𝐴 ⇛ 𝐵) v A = subsTyInProp 𝐴 v A ⇛ subsTyInProp 𝐵 v A
subsTyInProp (∀𝒳 𝐴) v A = ∀𝒳 (subsTyInProp 𝐴 v A)
subsTyInProp (∀x 𝐴) v A = ∀x (subsTyInProp 𝐴 v A)
subsTyInProp {Γ̂ = Γ̂} {Γ} (∀X 𝐴) v A =
  ∀X (tr (λ Γ̂ → Proposition Γ̂ (shiftCtx 𝑧𝑝 (subsCtx Γ v A))) (shiftSubsCtx v 𝑧𝑝 Γ̂ A)
    (tr (λ Γ → Proposition (subsCtx (shiftCtx 𝑧𝑝 Γ̂) (𝑠𝑣 v) A) Γ) (shiftSubsCtx v 𝑧𝑝 Γ A)
      (subsTyInProp 𝐴 (𝑠𝑣 v) A)))
